wip pipeline

compiler/src/PipelineWithRename.v
@@ -38,6 +38,9 @@ Require Import compiler.EventLoop.
 Require Import bedrock2.MetricLogging.
 Require Import compiler.FlatToRiscvCommon.
 Require Import compiler.FlatToRiscvFunctions.
+Require Import compiler.DivisibleBy4.
+Require Import compiler.SimplWordExpr.
+Require Import compiler.ForeverSafe.
 
 Existing Instance riscv.Spec.Machine.DefaultRiscvState.
 
@@ -135,13 +138,31 @@ Section Pipeline1.
     | None => FlatImp.SSkip
     end.
 
+  Local Notation cmd := (@Syntax.cmd (FlattenExpr.FlattenExpr.mk_Syntax_params _)).
+  Local Notation env := (@Semantics.env (FlattenExpr.mk_Semantics_params _)).
+
+  Lemma exprImp2Riscv_correct: forall (e: env) (sH: cmd) lH mH mcH t instsL
+                                      (initialL: MetricRiscvMachine) post,
+      @ExprImp.cmd_size (FlattenExpr.mk_Semantics_params _) sH < 2 ^ 10 ->
+      ExprImp2Riscv sH = instsL ->
+      (word.unsigned initialL.(getPc)) mod 4 = 0 ->
+      initialL.(getNextPc) = word.add initialL.(getPc) (word.of_Z 4) ->
+      initialL.(getLog) = t ->
+      (program initialL.(getPc) instsL * eq mH)%sep initialL.(getMem) ->
+      ext_guarantee initialL ->
+      Semantics.exec.exec e sH t mH lH mcH post ->
+      runsToNonDet.runsTo (mcomp_sat (run1 iset))
+             initialL
+             (fun finalL => exists mH' lH' mcH',
+                  post finalL.(getLog) mH' lH' mcH' /\
+                  (*map.extends finalL.(getRegs) lH' /\*)
+                  (program initialL.(getPc) (ExprImp2Riscv sH) * eq mH')%sep (getMem finalL)).
+  Admitted.
+
 (*
   Definition compile_functions(e: Semantics.env)(funnames: list funname): list Instruction :=
     FlatToRiscvDef.compile_functions (flatten_functions e funnames) funnames.
 *)
-
-  Local Notation cmd := (@Syntax.cmd (FlattenExpr.FlattenExpr.mk_Syntax_params _)).
-  Local Notation env := (@Semantics.env (FlattenExpr.mk_Semantics_params _)).
 
   Definition compile_prog(e: env) (init_sp: Z) (init_code loop_body: cmd)
              (funs: list funname): list Instruction :=
@@ -153,7 +174,12 @@ Section Pipeline1.
     FlatToRiscvDef.compile_lit RegisterNames.sp init_sp ++
     FlatToRiscvDef.compile_prog e'' init_code' loop_body' funs.
 
-  Lemma compile_prog_correct
+  Add Ring wring : (word.ring_theory (word := word))
+      (preprocess [autorewrite with rew_word_morphism],
+       morphism (word.ring_morph (word := word)),
+       constants [word_cst]).
+
+  Context
       (* high-level trace invariant which holds at the beginning of each loop iteration,
          but might not hold in the middle of the loop because more needs to be appended *)
       (hl_inv: trace -> Prop)
@@ -161,13 +187,87 @@ Section Pipeline1.
          loop iteration: *)
       (hl_ready: trace -> mem -> locals -> MetricLog -> Prop)
       (hl_ready_implies_hl_inv: forall t m l mc, hl_ready t m l mc -> hl_inv t)
-      (e: env) (t0: trace) (m0: mem) (l0: locals) (mc0: MetricLog)
+      (e: env) (t0: trace) (m0: mem) (l0: locals) (mc0: MetricLog) (st0: MetricRiscvMachine)
       (init_code loop_body: cmd)
       (funnames: list funname)
       (exec_init: Semantics.exec e init_code t0 m0 l0 mc0 hl_ready)
       (exec_body: forall t m l mc, hl_ready t m l mc ->
                                    Semantics.exec e loop_body t m l mc hl_ready)
-    :
+      (code_area_begin: word)
+      (code_area_begin_aligned: word.unsigned code_area_begin mod 4 = 0)
+      (insts_init: list Instruction)
+      (insts_body: list Instruction)
+      (* technical detail: "pc at beginning of loop" and "pc at end of loop" needs to be
+         different so that we can have two disjoint states between which the system goes
+         back and forth. If we had only one state, we could not prevent "runsTo" from
+         always being runsToDone and not making progress, see compiler.ForeverSafe *)
+      (insts_body_nonempty: insts_body <> nil).
+
+  (* pc at beginning of loop *)
+  Definition pc_start: word :=
+    word.add code_area_begin (word.of_Z (4 * Z.of_nat (List.length insts_init))).
+
+  Definition ll_ready(st: MetricRiscvMachine): Prop :=
+      exists regsH memH metricsH R p_stacklimit p_sp stack_trash initial_pc program_base
+      e_pos e_impl,
+        hl_ready st.(getLog) memH regsH metricsH /\
+        map.get st.(getRegs) RegisterNames.sp = Some p_sp /\
+        (R * eq memH * @word_array FlatToRisvc_params p_stacklimit stack_trash *
+         program initial_pc insts_init * program pc_start insts_body *
+         @functions FlatToRisvc_params program_base e_pos e_impl funnames)%sep st.(getMem).
+
+  Definition ll_inv: MetricRiscvMachine -> Prop := runsToGood_Invariant ll_ready pc_start.
+
+  Lemma ll_inv_is_invariant: forall st: MetricRiscvMachine,
+      ll_inv st -> mcomp_sat (run1 iset) st ll_inv.
+  Proof.
+    eapply runsToGood_is_Invariant with
+        (startState := st0)
+        (jump := - 4 * Z.of_nat (Datatypes.length insts_body))
+        (pc_end := word.add pc_start (word.of_Z (4 * Z.of_nat (List.length insts_body)))).
+    - intros. unfold ll_ready in *. simp. destruct_RiscvMachine state.
+      repeat match goal with
+             | |- exists _, _  => eexists
+             | |- _ /\ _ => split
+             | |- _ => eassumption
+             end.
+    - unfold pc_start. solve_divisibleBy4.
+    - admit.
+    - admit.
+    - solve_divisibleBy4.
+    - solve_word_eq word_ok.
+    - (* use compiler correctness for init_code *)
+      eapply runsTo_weaken.
+      + eapply exprImp2Riscv_correct; cycle -1.
+        1: exact exec_init.
+        all: try reflexivity; admit.
+      + simpl. intros. unfold ll_ready.
+        (* TODO: guarantee from exprImp2Riscv_correct needs to be stronger *)
+        admit.
+    - (* use compiler correctness for loop_body *)
+      intros.
+      eapply runsTo_weaken.
+      + unfold ll_ready in *. simp.
+        eapply exprImp2Riscv_correct; cycle -1.
+        1: { eapply exec_body. eassumption. }
+        all: try reflexivity; admit.
+      + simpl. intros. unfold ll_ready.
+        (* TODO: guarantee from exprImp2Riscv_correct needs to be stronger *)
+        admit.
+    all: fail.
+  Admitted.
+
+  Lemma ll_inv_implies_prefix_of_good: forall st,
+      ll_inv st -> exists suff, hl_inv (suff ++ st.(getLog)).
+  Proof.
+    unfold ll_inv, runsToGood_Invariant. intros.
+    eapply extend_runsTo_to_good_trace. 2: eassumption.
+    simpl. unfold ll_ready.
+    intros. simp.
+    eapply hl_ready_implies_hl_inv. eassumption.
+  Qed.
+
+  Lemma compile_prog_correct:
       (* there exists a low-level invariant which is somewhat complex and therefore not exposed *)
       exists ll_inv: MetricRiscvMachine -> Prop,
         (* how a client can establish ll_inv: *)
@@ -178,24 +278,6 @@ Section Pipeline1.
         (forall st: MetricRiscvMachine, ll_inv st -> mcomp_sat (run1 iset) st ll_inv /\
                                                      exists suff, hl_inv (suff ++ st.(getLog))).
   Proof.
-    intros.
-
-    assert (pc_start: word) by admit. (* start of loop body *)
-    assert (insts_init: list Instruction) by admit.
-    assert (insts_body: list Instruction) by admit.
-
-    set (ll_ready := fun (st: MetricRiscvMachine) =>
-      exists regsH memH metricsH R p_stacklimit p_sp stack_trash initial_pc program_base
-      e_pos e_impl,
-        hl_ready st.(getLog) memH regsH metricsH /\
-        map.get st.(getRegs) RegisterNames.sp = Some p_sp /\
-        (R * eq memH * @word_array FlatToRisvc_params p_stacklimit stack_trash *
-         program initial_pc insts_init * program pc_start insts_body *
-         @functions FlatToRisvc_params program_base e_pos e_impl funnames)%sep st.(getMem)).
-
-    pose proof (runsToGood_is_Invariant ll_ready) as P.
-    exists (runsToGood_Invariant ll_ready pc_start).
-
   Admitted.
 
 End Pipeline1.
